Validate list with int32. Switch to LowStar.Buffer

src/lowparse/LowParse.Low.Base.fst
@@ -1,8 +1,8 @@
 module LowParse.Low.Base
 include LowParse.Spec.Base
 
-module B = FStar.Buffer
-module M = FStar.Modifies
+module B = LowStar.Buffer
+module M = LowStar.Modifies
 module U32 = FStar.UInt32
 module HS = FStar.HyperStack
 module HST = FStar.HyperStack.ST
@@ -11,17 +11,28 @@ inline_for_extraction
 type buffer8 = B.buffer FStar.UInt8.t
 
 inline_for_extraction
-type pointer (t: Type) = (b: Buffer.buffer t { B.length b == 1 } )
+type pointer (t: Type) = (b: B.buffer t { B.length b == 1 } )
 
 module I32 = FStar.Int32
 
-let is_slice (h: HS.mem) (#t: Type) (b: Buffer.buffer t) (len: I32.t) : GTot Type0 =
+let is_slice (h: HS.mem) (#t: Type) (b: B.buffer t) (len: I32.t) : GTot Type0 =
   B.live h b /\
   B.length b == I32.v len
 
+unfold
+let gsub
+  (#t: Type)
+  (b: B.buffer t)
+  (i: U32.t)
+  (len: U32.t)
+: Ghost (B.buffer t)
+  (requires (U32.v i + U32.v len <= B.length b))
+  (ensures (fun b' -> B.length b' == U32.v len))
+= B.gsub b i len
+
 let is_tail_of (#t: Type) (b' b : B.buffer t) : GTot Type0 =
   B.length b' <= B.length b /\
-  b' == B.sub b (U32.uint_to_t (B.length b - B.length b')) (U32.uint_to_t (B.length b'))
+  b' == gsub b (U32.uint_to_t (B.length b - B.length b')) (U32.uint_to_t (B.length b'))
 
 let tail_ptr (h h' : HS.mem) (#t: Type) (p: pointer (B.buffer t)) : GTot Type0 =
   B.live h p /\
@@ -75,17 +86,6 @@ let exactly_parse_from_slice
     then Some x
     else None
   | _ -> None
-
-unfold
-let gsub
-  (#t: Type)
-  (b: B.buffer t)
-  (i: U32.t)
-  (len: U32.t)
-: Ghost (B.buffer t)
-  (requires (U32.v i + U32.v len <= B.length b))
-  (ensures (fun b' -> B.length b' == U32.v len))
-= B.sub b i len
 
 let exactly_parse_from_slice_intro'
   (#k: parser_kind)
@@ -209,161 +209,6 @@ let validator_nochk32
     let (Some (x, res')) = parse p (B.as_seq h input) in
     U32.v res == res'
   )))
-
-abstract
-let rec is_buffer_concat
-  (#t: Type)
-  (b: B.buffer t)
-  (l: list (B.buffer t))
-: GTot Type0
-  (decreases l)
-= match l with
-  | [] -> False
-  | [b'] -> b == b'
-  | b1 :: q ->
-    B.length b1 <= B.length b /\ (
-      let len1 = U32.uint_to_t (B.length b1) in
-      b1 == B.sub b 0ul len1 /\
-      B.sub b len1 (U32.uint_to_t (B.length b - B.length b1)) `is_buffer_concat` q
-    )
-
-abstract
-let is_buffer_concat_singleton
-  (#t: Type)
-  (b1 b2: B.buffer t)
-: Lemma
-  (is_buffer_concat b1 [b2] <==> b1 == b2)
-  [SMTPat (is_buffer_concat b1 [b2])]
-= ()
-
-abstract
-let is_buffer_concat_pair
-  (#t: Type)
-  (b b1 b2: B.buffer t)
-: Lemma
-  (is_buffer_concat b [b1; b2] <==> (
-    B.length b1 + B.length b2 == B.length b /\
-    b1 == B.sub b 0ul (U32.uint_to_t (B.length b1)) /\
-    b2 == B.sub b (U32.uint_to_t (B.length b1)) (U32.uint_to_t (B.length b2))
-  ))
-  [SMTPat (is_buffer_concat b [b1; b2])]
-= ()
-
-abstract
-let is_buffer_concat_cons
-  (#t: Type)
-  (b b1: B.buffer t)
-  (q: list (B.buffer t))
-: Lemma
-  (is_buffer_concat b (b1 :: q) <==> (
-    B.length b1 <= B.length b /\ (
-    let len1 = U32.uint_to_t (B.length b1) in
-    b1 == B.sub b 0ul len1 /\ (
-    if Cons? q
-    then
-      B.sub b len1 (U32.uint_to_t (B.length b - B.length b1)) `is_buffer_concat` q
-    else
-      b == b1
-  ))))
-  [SMTPat (is_buffer_concat b (b1 :: q))]
-= ()
-
-module L = FStar.List.Tot
-
-#set-options "--z3rlimit 16"
-
-abstract
-private
-let rec is_buffer_concat_subst_l
-  (#t: Type)
-  (b b': B.buffer t)
-  (l' l2: list (B.buffer t))
-: Lemma
-  (requires (
-    b `is_buffer_concat` (b' :: l2) /\
-    b' `is_buffer_concat` l'
-  ))
-  (ensures (
-    b `is_buffer_concat` (l' `L.append` l2)
-  ))
-  (decreases l')
-= match l' with
-  | [_] -> ()
-  | bq :: q ->
-    let len_bq = U32.uint_to_t (B.length bq) in
-    is_buffer_concat_subst_l
-      (B.sub b len_bq (U32.uint_to_t (B.length b - B.length bq)))
-      (B.sub b' len_bq (U32.uint_to_t (B.length b' - B.length bq)))
-      q
-      l2
-
-abstract
-let rec is_buffer_concat_subst
-  (#t: Type)
-  (b b': B.buffer t)
-  (l1 l' l2: list (B.buffer t))
-: Lemma
-  (requires (
-    b `is_buffer_concat` (l1 `L.append` (b' :: l2)) /\
-    b' `is_buffer_concat` l'
-  ))
-  (ensures (
-    b `is_buffer_concat` (l1 `L.append` (l' `L.append` l2))
-  ))
-  (decreases l1)
-= match l1 with
-  | [] -> is_buffer_concat_subst_l b b' l' l2
-  | bq :: q ->
-    let len_bq = U32.uint_to_t (B.length bq) in
-    is_buffer_concat_subst
-      (B.sub b len_bq (U32.uint_to_t (B.length b - B.length bq)))
-      b'
-      q
-      l'
-      l2
-
-abstract
-let rec is_buffer_concat_includes
-  (#t: Type)
-  (b b' : B.buffer t)
-  (l1 l2: list (B.buffer t))
-: Lemma
-  (requires (b `is_buffer_concat` (l1 `L.append` (b' :: l2))))
-  (ensures (b `B.includes` b'))
-  (decreases l1)
-= match l1 with
-  | [] -> ()
-  | bq :: q ->
-    is_buffer_concat_includes
-      (B.sub b (U32.uint_to_t (B.length bq)) (U32.uint_to_t (B.length b - B.length bq)))
-      b'
-      q
-      l2
-
-abstract
-let rec is_buffer_concat_disjoint
-  (#t: Type)
-  (b b1 b2: B.buffer t)
-  (l0 l1 l2: list (B.buffer t))
-: Lemma
-  (requires (b `is_buffer_concat` (l0 `L.append` (b1 :: (l1 `L.append` (b2 :: l2))))))
-  (ensures (B.disjoint b1 b2))
-  (decreases l0)
-= match l0 with
-  | [] ->
-    is_buffer_concat_includes
-      (B.sub b (U32.uint_to_t (B.length b1)) (U32.uint_to_t (B.length b - B.length b1)))
-      b2
-      l1
-      l2
-  | bq :: q ->
-    is_buffer_concat_disjoint
-      (B.sub b (U32.uint_to_t (B.length bq)) (U32.uint_to_t (B.length b - B.length bq)))
-      b1
-      b2
-      q
-      l1
-      l2
 
 inline_for_extraction
 let accessor
